library/init/data/ordering/basic.lean
@@ -11,6 +11,9 @@ universes u v
 inductive ordering
 | lt | eq | gt
 
+instance : has_repr ordering :=
+⟨(λ s, match s with | ordering.lt := "lt" | ordering.eq := "eq" | ordering.gt := "gt" end)⟩
+
 namespace ordering
 def swap : ordering → ordering
 | lt := gt
@@ -28,45 +31,30 @@ theorem swap_swap : ∀ (o : ordering), o.swap.swap = o
 | gt := rfl
 end ordering
 
-open ordering
-
-instance : has_repr ordering :=
-⟨(λ s, match s with | ordering.lt := "lt" | ordering.eq := "eq" | ordering.gt := "gt" end)⟩
-
-class has_cmp (α : Type u) :=
-(cmp : α → α → ordering)
-
-def cmp_of_lt {α : Type u} [has_lt α] [decidable_rel ((<) : α → α → Prop)] (a b : α) : ordering :=
-if      a < b then ordering.lt
+def cmp {α : Type u} [has_lt α] [decidable_rel ((<) : α → α → Prop)] (a b : α) : ordering :=
+if a < b then ordering.lt
 else if b < a then ordering.gt
-else               ordering.eq
+else ordering.eq
 
-instance has_cmp_of_lt {α : Type u} [has_lt α] [decidable_rel ((<) : α → α → Prop)] : has_cmp α :=
-⟨cmp_of_lt⟩
-
-/- Remark: this function has a VM builtin efficient implementation. -/
-protected def string.cmp (s1 s2 : string) : ordering :=
-cmp_of_lt s1 s2
-
-instance : has_cmp string :=
-⟨string.cmp⟩
-
-export has_cmp (cmp)
-
-section cmp_relations
-variables {α : Type u} [has_cmp α]
-
-@[reducible] def cmp_lt (a b : α) : Prop :=
-cmp a b = ordering.lt
-
-@[reducible] def cmp_eq (a b : α) : Prop :=
-cmp a b = ordering.eq
-
-@[reducible] def cmp_gt (a b : α) : Prop :=
-cmp a b = ordering.gt
-
-infix ` <_cmp `:50 := cmp_lt
-infix ` =_cmp `:50 := cmp_eq
-infix ` >_cmp `:50 := cmp_gt
-
-end cmp_relations
+instance : decidable_eq ordering :=
+λ a b,
+  match a with
+  | ordering.lt :=
+    match b with
+    | ordering.lt := is_true rfl
+    | ordering.eq := is_false (λ h, ordering.no_confusion h)
+    | ordering.gt := is_false (λ h, ordering.no_confusion h)
+    end
+  | ordering.eq :=
+    match b with
+    | ordering.lt := is_false (λ h, ordering.no_confusion h)
+    | ordering.eq := is_true rfl
+    | ordering.gt := is_false (λ h, ordering.no_confusion h)
+    end
+  | ordering.gt :=
+    match b with
+    | ordering.lt := is_false (λ h, ordering.no_confusion h)
+    | ordering.eq := is_false (λ h, ordering.no_confusion h)
+    | ordering.gt := is_true rfl
+    end
+  end
